Revert "turned out we had a useless layer"
This reverts commit 645610052f4c0ae316575e6c36bad8d242267b10.

src/Mail2/TryDeliverImpl.v
@@ -2,7 +2,7 @@ Require Import POCS.
 Require Import String.
 Require Import MailServerAPI.
 Require Import MailboxAPI.
-Require Import DeliverAPI.
+Require Import TryDeliverAPI.
 Require Import MailFSAPI.
 Require Import MailboxTmpAbsAPI.
 
@@ -11,24 +11,24 @@ Module TryDeliverImpl' <:
   LayerImplMoversT
     MailboxTmpAbsState
     MailFSOp     MailFSAPI
-    DeliverOp    DeliverAPI.
+    TryDeliverOp TryDeliverAPI.
 
   Definition linkmail_core :=
     ts <- Op MailFSOp.Random;
     ok <- Op (MailFSOp.LinkMail ts);
     Ret ok.
 
-  Definition compile_op T (op : DeliverOp.opT T) : proc MailFSOp.opT T :=
+  Definition compile_op T (op : TryDeliverOp.opT T) : proc MailFSOp.opT T :=
     match op with
-    | DeliverOp.CreateWriteTmp data => Op (MailFSOp.CreateWriteTmp data)
-    | DeliverOp.LinkMail => linkmail_core
-    | DeliverOp.UnlinkTmp => Op (MailFSOp.UnlinkTmp)
-    | DeliverOp.List => Op (MailFSOp.List)
-    | DeliverOp.Read fn => Op (MailFSOp.Read fn)
-    | DeliverOp.Delete fn => Op (MailFSOp.Delete fn)
-    | DeliverOp.Lock => Op (MailFSOp.Lock)
-    | DeliverOp.Unlock => Op (MailFSOp.Unlock)
-    | DeliverOp.Ext extop => Op (MailFSOp.Ext extop)
+    | TryDeliverOp.CreateWriteTmp data => Op (MailFSOp.CreateWriteTmp data)
+    | TryDeliverOp.LinkMail => linkmail_core
+    | TryDeliverOp.UnlinkTmp => Op (MailFSOp.UnlinkTmp)
+    | TryDeliverOp.List => Op (MailFSOp.List)
+    | TryDeliverOp.Read fn => Op (MailFSOp.Read fn)
+    | TryDeliverOp.Delete fn => Op (MailFSOp.Delete fn)
+    | TryDeliverOp.Lock => Op (MailFSOp.Lock)
+    | TryDeliverOp.Unlock => Op (MailFSOp.Unlock)
+    | TryDeliverOp.Ext extop => Op (MailFSOp.Ext extop)
     end.
 
   Theorem compile_op_no_atomics :
@@ -40,13 +40,13 @@ Module TryDeliverImpl' <:
 
   Ltac step_inv :=
     match goal with
-    | H : DeliverAPI.step _ _ _ _ _ _ |- _ =>
+    | H : TryDeliverAPI.step _ _ _ _ _ _ |- _ =>
       inversion H; clear H; subst; repeat sigT_eq
     | H : MailFSAPI.step _ _ _ _ _ _ |- _ =>
       inversion H; clear H; subst; repeat sigT_eq
     end; intuition idtac.
 
-  Hint Extern 1 (DeliverAPI.step _ _ _ _ _ _) => econstructor.
+  Hint Extern 1 (TryDeliverAPI.step _ _ _ _ _ _) => econstructor.
   Hint Extern 1 (MailFSAPI.step _ _ _ _ _ _) => econstructor.
 
   Lemma random_right_mover :
@@ -77,7 +77,7 @@ Module TryDeliverImpl' <:
   Qed.
 
   Theorem compile_correct :
-    compile_correct compile_op MailFSAPI.step DeliverAPI.step.
+    compile_correct compile_op MailFSAPI.step TryDeliverAPI.step.
   Proof.
     unfold compile_correct; intros.
     destruct op.
@@ -92,14 +92,14 @@ Module TryDeliverImpl :=
   LayerImplMovers
     MailboxTmpAbsState
     MailFSOp     MailFSAPI
-    DeliverOp    DeliverAPI
+    TryDeliverOp TryDeliverAPI
     TryDeliverImpl'.
 
 Module TryDeliverImplH' :=
   LayerImplMoversHT
     MailboxTmpAbsState
     MailFSOp     MailFSAPI
-    DeliverOp    DeliverAPI
+    TryDeliverOp TryDeliverAPI
     TryDeliverImpl'
     UserIdx.
 
@@ -107,5 +107,5 @@ Module TryDeliverImplH :=
   LayerImplMovers
     MailboxTmpAbsHState
     MailFSHOp     MailFSHAPI
-    DeliverHOp    DeliverHAPI
+    TryDeliverHOp TryDeliverHAPI
     TryDeliverImplH'.
