src/Mail2/LinkRetryImpl.v
@@ -1,0 +1,79 @@
+Require Import POCS.
+Require Import String.
+Require Import MailServerAPI.
+Require Import MailboxAPI.
+Require Import MailboxTmpAbsAPI.
+Require Import DeliverAPI.
+Require Import TryDeliverAPI.
+
+
+Module LinkRetryImpl' <:
+  LayerImplLoopT
+    MailboxTmpAbsState
+    TryDeliverOp TryDeliverAPI
+    DeliverOp DeliverAPI.
+
+  Definition retry_cond (r : bool) := r.
+  Definition once_cond {T} (r : T) := true.
+
+  Definition compile_op T (op : DeliverOp.opT T) : (option T -> TryDeliverOp.opT T) * (T -> bool) * option T :=
+    match op with
+    | DeliverOp.CreateWriteTmp data => (fun _ => TryDeliverOp.CreateWriteTmp data, once_cond, None)
+    | DeliverOp.LinkMail => (fun _ => TryDeliverOp.LinkMail, retry_cond, None)
+    | DeliverOp.UnlinkTmp => (fun _ => TryDeliverOp.UnlinkTmp, once_cond, None)
+    | DeliverOp.List => (fun _ => TryDeliverOp.List, once_cond, None)
+    | DeliverOp.Read fn => (fun _ => TryDeliverOp.Read fn, once_cond, None)
+    | DeliverOp.Delete fn => (fun _ => TryDeliverOp.Delete fn, once_cond, None)
+    | DeliverOp.Lock => (fun _ => TryDeliverOp.Lock, once_cond, None)
+    | DeliverOp.Unlock => (fun _ => TryDeliverOp.Unlock, once_cond, None)
+    | DeliverOp.Ext extop => (fun _ => TryDeliverOp.Ext extop, once_cond, None)
+    end.
+
+  Ltac step_inv :=
+    match goal with
+    | H : TryDeliverAPI.xstep _ _ _ _ _ _ |- _ =>
+      inversion H; clear H; subst; repeat sigT_eq
+    | H : DeliverAPI.xstep _ _ _ _ _ _ |- _ =>
+      inversion H; clear H; subst; repeat sigT_eq
+    end.
+
+  Ltac pair_inv :=
+    match goal with
+    | H : (_, _) = (_, _) |- _ =>
+      inversion H; clear H; subst; repeat sigT_eq
+    end.
+
+  Hint Constructors TryDeliverAPI.xstep.
+  Hint Constructors DeliverAPI.xstep.
+
+  Theorem noop_or_success :
+    noop_or_success compile_op TryDeliverAPI.step DeliverAPI.step.
+  Proof.
+    unfold noop_or_success.
+    unfold TryDeliverAPI.step, DeliverAPI.step.
+    destruct opM; simpl; intros; pair_inv; step_inv; eauto.
+  Qed.
+
+End LinkRetryImpl'.
+
+Module LinkRetryImpl :=
+  LayerImplLoop
+    MailboxTmpAbsState
+    TryDeliverOp TryDeliverAPI
+    DeliverOp DeliverAPI
+    LinkRetryImpl'.
+
+Module LinkRetryImplH' :=
+  LayerImplLoopHT
+    MailboxTmpAbsState
+    TryDeliverOp TryDeliverAPI
+    DeliverOp DeliverAPI
+    LinkRetryImpl'
+    UserIdx.
+
+Module LinkRetryImplH :=
+  LayerImplLoop
+    MailboxTmpAbsHState
+    TryDeliverHOp TryDeliverHAPI
+    DeliverHOp DeliverHAPI
+    LinkRetryImplH'.
