src/Mail2/MailServer.v
@@ -33,6 +33,9 @@ Require Import MailFSPathAbsImpl.
 Require Import MailFSPathAPI.
 Require Import MailFSPathImpl.
 
+Require Import LinkRetryImpl.
+
+Require Import TryDeliverAPI.
 Require Import TryDeliverImpl.
 
 Require Import MailFSMergedAPI.
@@ -207,12 +210,18 @@ Module c5 :=
     MailServerHOp     MailServerHState    MailServerHAPI
     MailFSImplH c4.
 
-Module c45' :=
+Module c4' :=
   Link
-    MailFSHOp     MailboxTmpAbsHState MailFSHAPI
+    TryDeliverHOp MailboxTmpAbsHState TryDeliverHAPI
     DeliverHOp    MailboxTmpAbsHState DeliverHAPI
     MailServerHOp MailServerHState    MailServerHAPI
-    TryDeliverImplH c3.
+    LinkRetryImplH c3.
+Module c5' :=
+  Link
+    MailFSHOp     MailboxTmpAbsHState MailFSHAPI
+    TryDeliverHOp MailboxTmpAbsHState TryDeliverHAPI
+    MailServerHOp MailServerHState    MailServerHAPI
+    TryDeliverImplH c4'.
 
 Module c6 :=
   Link
@@ -221,7 +230,7 @@ Module c6 :=
     MailServerHOp MailServerHState      MailServerHAPI
     MailFSStringAbsImplH
     (* c5 *)
-    c45'.
+    c5'.
 
 Module c7 :=
   Link
